@prefix rdf: <http://www.w3.org/1999/02/22-rdf-syntax-ns#> .
@prefix rdfs: <http://www.w3.org/2000/01/rdf-schema#> .
@prefix xsd: <http://www.w3.org/2001/XMLSchema#> .


#
# ╭──────────────────────────────────────────────────╮
# │ Class: GitCommit                                 │
# ╰──────────────────────────────────────────────────╯
#
:GitCommit a rdfs:Class ;
    rdfs:label "Git Commit"@en ;
    rdfs:comment "Represents a Git-Commit."@en .

# GitCommit properties

:authorName a rdf:Property ;
    rdfs:label "AuthorName"@en ;
    rdfs:comment "The name of the author for this commit (git config user.name)."@en ;
    rdfs:domain :GitCommit ;
    rdfs:range xsd:string .

:authorEmail a rdf:Property ;
    rdfs:label "AuthorEmail"@en ;
    rdfs:comment "The email of the author for this commit (git config user.email)."@en ;
    rdfs:domain :GitCommit ;
    rdfs:range xsd:string .

:authorDate a rdf:Property ;
    rdfs:label "AuthorDate"@en ;
    rdfs:comment "A timestamp of the commit from the author."@en ;
    rdfs:domain :GitCommit ;
    rdfs:range xsd:dateTime .

:commitDate a rdf:Property ;
    rdfs:label "CommitDate"@en ;
    rdfs:comment "A timestamp of the commit from the committer."@en ;
    rdfs:domain :GitCommit ;
    rdfs:range xsd:dateTime .

:committerName a rdf:Property ;
    rdfs:label "CommitterName"@en ;
    rdfs:comment "The name of the committer (git config user.name)."@en ;
    rdfs:domain :GitCommit ;
    rdfs:range xsd:string .

:committerEmail a rdf:Property ;
    rdfs:label "CommitterEmail"@en ;
    rdfs:comment "The email of the committer (git config user.email)"@en ;
    rdfs:domain :GitCommit ;
    rdfs:range xsd:string .

:commitMessage a rdf:Property ;
    rdfs:label "CommitMessage"@en ;
    rdfs:comment "The commit-message for this commit."@en ;
    rdfs:domain :GitCommit ;
    rdfs:range xsd:string .

:branchName a rdf:Property ;
    rdfs:label "BranchName"@en ;
    rdfs:comment "A name of a branch where this commit is in (includes also merged branches)."@en ;
    rdfs:domain :GitCommit ;
    rdfs:range xsd:string .

:diffEntry a rdf:Property ;
    rdfs:label "DiffEntry"@en ;
    rdfs:comment "An entry for a diff compared to the parent of the commit."@en ;
    rdfs:domain :GitCommit ;
    rdfs:range :CommitDiffEntry .

#
# ╭──────────────────────────────────────────────────╮
# │ Class: CommitDiffEntry                           │
# ╰──────────────────────────────────────────────────╯
#
:CommitDiffEntry a rdfs:Class ;
    rdfs:label "Commit Diff Entry"@en ;
    rdfs:comment "A diff-entry is usually a single file where one or multiple changes in a commit were applied compared to the parent-commit of the commit. Can also represent added or removed files, depending on the <ChangeType>."@en ;
    rdfs:domain :GitCommit .

# CommitDiffEntry properties

:changeType a rdf:Property ;
    rdfs:label "ChangeType"@en ;
    rdfs:comment "Spezifies the type of the diff-entry. Can be modified files or added/removed files."@en ;
    rdfs:domain :CommitDiffEntry ;
    rdfs:range :ChangeType .

:oldFileName a rdf:Property ;
    rdfs:label "OldFileName"@en ;
    rdfs:comment "The name of the file (complete relative path) of the parent-commit where changes occur. If the filename has not changed, the original filename is contained in here."@en ;
    rdfs:domain :CommitDiffEntry ;
    rdfs:range xsd:string .

:newFileName a rdf:Property ;
    rdfs:label "NewFileName"@en ;
    rdfs:comment "The filename (complete relative path) of the new file, in case a file has been renamed or added."@en ;
    rdfs:domain :CommitDiffEntry ;
    rdfs:range xsd:string .

:edit a rdf:Property ;
    rdfs:label "Edit"@en ;
    rdfs:comment "Represents a section of lines which have added, deleted or modified within a file."@en ;
    rdfs:domain :CommitDiffEntry ;
    rdfs:range :CommitDiffEdit .


#
# ╭──────────────────────────────────────────────────╮
# │ Class: CommitDiffEdit                            │
# ╰──────────────────────────────────────────────────╯
#
:CommitDiffEdit a rdfs:Class ;
    rdfs:label "Commit Diff Entry Edit"@en ;
    rdfs:comment "A section of lines which have been added, deleted or modified within a file."@en .

# CommitDiffEdit properties

:editType a rdf:Property ;
    rdfs:label "EditType"@en ;
    rdfs:comment "The kind of edit that has taken place (insert/delete/replace), see <EditType>."@en ;
    rdfs:domain :CommitDiffEdit ;
    rdfs:range :EditType .

:oldLinenumberBegin a rdf:Property ;
    rdfs:label "OldLinenumberBegin"@en ;
    rdfs:comment "The line number beginning from 0 in the diff of the parent commit where a section has been edited."@en ;
    rdfs:domain :CommitDiffEdit ;
    rdfs:range xsd:integer .

:newLinenumberBegin a rdf:Property ;
    rdfs:label "NewLinenumberBegin"@en ;
    rdfs:comment "The line number beginning from 0 in the diff of the current commit where a section has been edited."@en ;
    rdfs:domain :CommitDiffEdit ;
    rdfs:range xsd:integer .

:oldLinenumberEnd a rdf:Property ;
    rdfs:label "OldLinenumberEnd"@en ;
    rdfs:comment "The line number ending in the diff of the parent commit where a section has been edited."@en ;
    rdfs:domain :CommitDiffEdit ;
    rdfs:range xsd:integer .

:newLinenumberEnd a rdf:Property ;
    rdfs:label "NewLinenumberEnd"@en ;
    rdfs:comment "The line number ending in the diff of the current commit where a section has been edited."@en ;
    rdfs:domain :CommitDiffEdit ;
    rdfs:range xsd:integer .

#
# ╭──────────────────────────────────────────────────╮
# │ Enumeration: ChangeType                          │
# ╰──────────────────────────────────────────────────╯
#
:ChangeType a rdfs:Class ;
    rdfs:label "Change Type"@en ;
    rdfs:comment "Specifies the changes of a DiffEntry (usually for a file) that have been modified."@en .

:add a :ChangeType ;
    rdfs:label "Add"@en ;
    rdfs:comment "A file has been added."@en .

:delete a :ChangeType ;
    rdfs:label "Delete"@en ;
    rdfs:comment "A file has been deleted."@en .

:modify a :ChangeType ;
    rdfs:label "Modify"@en ;
    rdfs:comment "A file has been modified."@en .

:rename a :ChangeType ;
    rdfs:label "Rename"@en ;
    rdfs:comment "A file has been renamed."@en .

:copy a :ChangeType ;
    rdfs:label "Copy"@en ;
    rdfs:comment "A file has been copied."@en .

#
# ╭──────────────────────────────────────────────────╮
# │ Enumeration: EditType                            │
# ╰──────────────────────────────────────────────────╯
#
:EditType a rdfs:Class ;
    rdfs:label "Edit Type"@en ;
    rdfs:comment "Specifies the kind of edit within a DiffEntry/file for a section of text-lines."@en .

:insert a :EditType ;
    rdfs:label "Insert"@en ;
    rdfs:comment "Content has been added/inserted into a file."@en .

:del a :EditType ;
    rdfs:label "Delete"@en ;
    rdfs:comment "Content has been removed/deleted from a file."@en .

:replace a :EditType ;
    rdfs:label "Replace"@en ;
    rdfs:comment "Content has been replaced within a file."@en .


